Correct spec: And/Or in subject matches is a list

com.io7m.medrina.documentation/src/main/coq/Medrina/Matches.v
@@ -15,6 +15,9 @@
  *)
 
 Require Import Coq.Strings.String.
+Require Import Coq.Lists.List.
+
+Import ListNotations.
 
 Require Import Medrina.Actions.
 Require Import Medrina.Names.
@@ -24,23 +27,41 @@ Require Import Medrina.Objects.
 
 (** An expression that matches a subject. *)
 Inductive exprMatchSubject : Type :=
-  | EMS_False : exprMatchSubject
-  | EMS_True : exprMatchSubject
-  | EMS_WithRolesAll :
-    forall (r : RoleSets.t),
-      exprMatchSubject
-  | EMS_WithRolesAny :
-    forall (r : RoleSets.t),
-      exprMatchSubject
-  | EMS_And :
-    exprMatchSubject ->
-      exprMatchSubject ->
-        exprMatchSubject
-  | EMS_Or :
-    exprMatchSubject ->
-      exprMatchSubject ->
-        exprMatchSubject
+  | EMS_False        : exprMatchSubject
+  | EMS_True         : exprMatchSubject
+  | EMS_WithRolesAll : RoleSets.t -> exprMatchSubject
+  | EMS_WithRolesAny : RoleSets.t -> exprMatchSubject
+  | EMS_And          : list exprMatchSubject -> exprMatchSubject
+  | EMS_Or           : list exprMatchSubject -> exprMatchSubject
   .
+
+Section ExprMatchSubjects_ind.
+  Variable P : exprMatchSubject -> Prop.
+  Hypothesis P_False        : P EMS_False.
+  Hypothesis P_True         : P EMS_True.
+  Hypothesis P_WithRolesAll : forall r, P (EMS_WithRolesAll r).
+  Hypothesis P_WithRolesAny : forall r, P (EMS_WithRolesAny r).
+  Hypothesis P_And          : forall es, Forall P es -> P (EMS_And es).
+  Hypothesis P_Or           : forall es, Forall P es -> P (EMS_Or es).
+
+  Fixpoint exprMatchSubject_extendedInd (e : exprMatchSubject) : P e :=
+    let
+      fix e_list (xs : list exprMatchSubject) : Forall P xs :=
+        match xs as rxs return (Forall P rxs) with
+        | []        => Forall_nil _
+        | (y :: ys) => @Forall_cons _ _ y ys (exprMatchSubject_extendedInd y) (e_list ys)
+        end
+    in
+      match e with
+      | EMS_False          => P_False
+      | EMS_True           => P_True
+      | EMS_WithRolesAll r => P_WithRolesAll r
+      | EMS_WithRolesAny r => P_WithRolesAny r
+      | EMS_And es         => P_And es (e_list es)
+      | EMS_Or es          => P_Or es (e_list es)
+      end.
+
+End ExprMatchSubjects_ind.
 
 (** An evaluation function for subject match expressions. *)
 Fixpoint exprMatchSubjectEvalF
@@ -48,185 +69,426 @@ Fixpoint exprMatchSubjectEvalF
   (e : exprMatchSubject)
 : bool :=
   match e with
-  | EMS_False => false
-  | EMS_True => true
-  | EMS_WithRolesAll r =>
-    RoleSets.subset r (sRoles s)
-  | EMS_WithRolesAny r =>
-    RoleSets.exists_ (fun x => RoleSets.mem x (sRoles s)) r
-  | EMS_And x y =>
-    andb (exprMatchSubjectEvalF s x) (exprMatchSubjectEvalF s y)
-  | EMS_Or x y =>
-    orb (exprMatchSubjectEvalF s x) (exprMatchSubjectEvalF s y)
+  | EMS_False          => false
+  | EMS_True           => true
+  | EMS_WithRolesAll r => RoleSets.subset r (sRoles s)
+  | EMS_WithRolesAny r => RoleSets.exists_ (fun x => RoleSets.mem x (sRoles s)) r
+  | EMS_And es         => forallb (exprMatchSubjectEvalF s) es
+  | EMS_Or es          => existsb (exprMatchSubjectEvalF s) es
   end.
 
 (** The evaluation function for subject match expressions as a relation. *)
-Inductive exprMatchSubjectEvalR : subject -> exprMatchSubject -> Prop :=
+Inductive exprMatchSubjectEvalR (s : subject) : exprMatchSubject -> Prop :=
   | EMSR_True :
-    forall (s : subject),
       exprMatchSubjectEvalR s EMS_True
   | EMSR_WithRolesAll :
-    forall (s : subject) (r : RoleSets.t),
+    forall (r : RoleSets.t),
       RoleSets.Subset r (sRoles s) ->
         exprMatchSubjectEvalR s (EMS_WithRolesAll r)
   | EMSR_WithRolesAny :
-    forall (s : subject) (r : RoleSets.t),
+    forall (r : RoleSets.t),
       (exists x, RoleSets.In x r /\ RoleSets.In x (sRoles s)) ->
         exprMatchSubjectEvalR s (EMS_WithRolesAny r)
   | EMSR_And :
-    forall (s : subject) (e0 e1 : exprMatchSubject),
-      exprMatchSubjectEvalR s e0 /\ exprMatchSubjectEvalR s e1 ->
-        exprMatchSubjectEvalR s (EMS_And e0 e1)
+    forall (es : list exprMatchSubject),
+      Forall (exprMatchSubjectEvalR s) es ->
+        exprMatchSubjectEvalR s (EMS_And es)
   | EMSR_Or :
-    forall (s : subject) (e0 e1 : exprMatchSubject),
-      exprMatchSubjectEvalR s e0 \/ exprMatchSubjectEvalR s e1 ->
-        exprMatchSubjectEvalR s (EMS_Or e0 e1)
+    forall (e : exprMatchSubject) (es : list exprMatchSubject),
+      Exists (exprMatchSubjectEvalR s) (e :: es) ->
+        exprMatchSubjectEvalR s (EMS_Or (e :: es))
   .
+
+(** Implication lifted into the Forall structure. *)
+Lemma Forall_impl_lifted : forall
+  (A  : Type)
+  (P  : A -> Prop)
+  (Q  : A -> Prop)
+  (xs : list A),
+  Forall (fun x => P x) xs ->
+    Forall (fun x => P x -> Q x) xs ->
+      Forall (fun x => Q x) xs.
+Proof.
+  induction xs as [|y ys IH]. {
+    intros F0 H1.
+    constructor.
+  } {
+    intros F0 F1.
+    constructor. {
+      apply (Forall_inv F1).
+      apply (Forall_inv F0).
+    } {
+      apply IH.
+      apply (Forall_inv_tail F0).
+      apply (Forall_inv_tail F1).
+    }
+  }
+Qed.
+
+Lemma exprMatchSubjectEvalEquivalent_FR_T : forall s e,
+  true = exprMatchSubjectEvalF s e -> exprMatchSubjectEvalR s e.
+Proof.
+  intros s e.
+  induction e as [
+    |
+    |
+    |
+    |es Hes
+    |es Hes
+  ] using exprMatchSubject_extendedInd. {
+    (* EMS_False *)
+    intros Ht.
+    inversion Ht.
+  } {
+    (* EMS_True *)
+    intros Ht.
+    constructor.
+  } {
+    (* EMS_WithRolesAll *)
+    intros Ht.
+    unfold exprMatchSubjectEvalF in Ht.
+    constructor.
+    apply RoleSets.subset_2.
+    intuition.
+  } {
+    (* EMS_WithRolesAny *)
+    intros Ht.
+    unfold exprMatchSubjectEvalF in Ht.
+    constructor.
+    symmetry in Ht.
+
+    assert (
+      SetoidList.compat_bool
+        RoleSets.E.eq (fun x : RoleSets.elt => RoleSets.mem x (sRoles s))
+    ) as Hsetcomp. {
+      unfold SetoidList.compat_bool.
+      unfold Morphisms.Proper.
+      unfold Morphisms.respectful.
+      intros x y Heq.
+      rewrite Heq.
+      reflexivity.
+    }
+
+    pose proof (RoleSets.exists_2 Hsetcomp Ht) as [x [H0 H1]].
+    exists x.
+    intuition.
+  } {
+    (* EMS_And *)
+    destruct es as [|y ys]. {
+      intros Ht.
+      constructor.
+      constructor.
+    } {
+      simpl.
+      intros Ht.
+
+      (* We need to show that the relation holds for all (y :: ys). *)
+      assert (Forall (exprMatchSubjectEvalR s) (y :: ys)) as H0. {
+        (* We do this by showing it holds for y... *)
+        assert (exprMatchSubjectEvalR s y) as H1. {
+          symmetry in Ht.
+          rewrite Bool.andb_true_iff in Ht.
+          rewrite forallb_forall in Ht.
+          destruct Ht as [HT0 HT1].
+          rewrite <- (@Forall_forall exprMatchSubject _ ys) in HT1.
+
+          apply (Forall_inv Hes).
+          symmetry.
+          exact HT0.
+        }
+
+        (* ... And for all ys. *)
+        assert (Forall (exprMatchSubjectEvalR s) ys) as H2. {
+          symmetry in Ht.
+          rewrite Bool.andb_true_iff in Ht.
+          rewrite forallb_forall in Ht.
+          destruct Ht as [HT0 HT1].
+          rewrite <- (@Forall_forall exprMatchSubject _ ys) in HT1.
+
+          assert (Forall (fun x : exprMatchSubject => true = exprMatchSubjectEvalF s x) ys) as H2. {
+            rewrite Forall_forall.
+            symmetry.
+            generalize dependent x.
+            rewrite <- Forall_forall.
+            exact HT1.
+          }
+
+          pose proof (Forall_inv_tail Hes) as HesT.
+          apply (Forall_impl_lifted _ _ _ ys H2 HesT).
+        }
+
+        (* ... And then composing the two. *)
+        constructor.
+        exact H1.
+        exact H2.
+      }
+
+      constructor.
+      exact H0.
+    }
+  } {
+    (* EMS_Or *)
+    destruct es as [|y ys]. {
+      intros Ht.
+      contradict Ht. simpl. discriminate.
+    } {
+      intros Ht.
+
+      (* We need to show that the relation holds for y or something in ys. *)
+      constructor.
+
+      simpl in Ht.
+      symmetry in Ht.
+      destruct (Bool.orb_true_elim _ _ Ht) as [HtL|HtR]. {
+        constructor.
+        apply (Forall_inv Hes).
+        auto.
+      } {
+        assert (Exists (exprMatchSubjectEvalR s) (y :: ys)) as H0. {
+          rewrite existsb_exists in HtR.
+          destruct HtR as [k [Htk0 Htk1]].
+          rewrite Forall_forall in Hes.
+          pose proof (in_cons y k ys Htk0) as H0.
+          pose proof (Hes k H0 (eq_sym Htk1)) as H1.
+          apply Exists_cons_tl.
+          rewrite Exists_exists.
+          exists k.
+          auto.
+        }
+        exact H0.
+      }
+    }
+  }
+Qed.
+
+Lemma  exprMatchSubjectEvalEquivalent_RF_T : forall s e,
+  exprMatchSubjectEvalR s e -> true = exprMatchSubjectEvalF s e.
+Proof.
+  intros s e.
+  induction e as [
+    |
+    |
+    |
+    |es Hes
+    |es Hes
+  ] using exprMatchSubject_extendedInd. {
+    (* EMS_False *)
+    intros Ht.
+    inversion Ht.
+  } {
+    (* EMS_True *)
+    intros Ht.
+    reflexivity.
+  } {
+    (* EMS_WithRolesAll *)
+    intros Ht.
+    symmetry.
+    apply RoleSets.subset_1.
+    inversion Ht.
+    intuition.
+  } {
+    (* EMS_WithRolesAny *)
+    intros Ht.
+    symmetry.
+    inversion Ht as [ | |s0 Hexist Heq| | ].
+    subst s0.
+    simpl.
+    assert (
+      RoleSets.Exists
+        (fun x : RoleSets.elt => RoleSets.mem x (sRoles s) = true) r
+    ) as Hex. {
+      unfold RoleSets.Exists.
+      destruct Hexist as [y [Hy0 Hy1]].
+      exists y.
+      intuition.
+    }
+
+    assert (
+      SetoidList.compat_bool
+        RoleSets.E.eq (fun x : RoleSets.elt => RoleSets.mem x (sRoles s))
+    ) as Hsetcomp. {
+      unfold SetoidList.compat_bool.
+      unfold Morphisms.Proper.
+      unfold Morphisms.respectful.
+      intros x y Heq.
+      rewrite Heq.
+      reflexivity.
+    }
+
+    apply (RoleSets.exists_1 Hsetcomp Hex).
+  } {
+    (* EMS_And *)
+    intros Ht.
+    inversion Ht as [ | | |es0 Hfa Heq|].
+    subst es0.
+    simpl.
+    symmetry.
+    rewrite forallb_forall.
+    intros x Hin.
+    symmetry.
+    generalize dependent x.
+    rewrite <- Forall_forall.
+    apply (Forall_impl_lifted exprMatchSubject _ _ es Hfa Hes).
+  } {
+    (* EMS_Or *)
+    intros Ht.
+    symmetry.
+    simpl.
+    rewrite existsb_exists.
+
+    inversion Ht as [ | | | |e es0 Hex Heq].
+    subst es.
+    destruct Hex as [k ks Hk|k ks Hk]. {
+      exists k.
+      constructor.
+      constructor; reflexivity.
+      apply (eq_sym (Forall_inv Hes Hk)).
+    } {
+      rewrite Exists_exists in Hk.
+      destruct Hk as [q [Hq0 Hq1]].
+      exists q.
+      constructor.
+      apply (in_cons k q ks Hq0).
+      pose proof (Forall_inv_tail Hes) as HesT.
+      rewrite Forall_forall in HesT.
+      apply (eq_sym (HesT q Hq0 Hq1)).
+    }
+  }
+Qed.
 
 (** The evaluation function and the evaluation relation are equivalent. *)
 Theorem exprMatchSubjectEvalEquivalentT : forall s e,
   true = exprMatchSubjectEvalF s e <-> exprMatchSubjectEvalR s e.
 Proof.
+  split.
+  apply exprMatchSubjectEvalEquivalent_FR_T.
+  apply exprMatchSubjectEvalEquivalent_RF_T.
+Qed.
+
+Lemma exprMatchSubjectEvalEquivalent_FR_F : forall s e,
+  false = exprMatchSubjectEvalF s e -> ~exprMatchSubjectEvalR s e.
+Proof.
   intros s e.
   induction e as [
     |
-    |r
-    |r
-    |e0 He0 e1 He1
-    |e0 He0 e1 He1
-  ]. {
+    |
+    |
+    |es Hes
+    |es Hes
+  ] using exprMatchSubject_extendedInd. {
     (* EMS_False *)
-    split. {
-      intros Ht.
-      inversion Ht.
-    } {
-      intros Ht.
-      inversion Ht.
-    }
+    intros Ht.
+    intro Hcontra.
+    inversion Hcontra.
   } {
     (* EMS_True *)
-    split. {
-      intros Ht; constructor.
-    } {
-      intros Ht; reflexivity.
-    }
+    intros Ht.
+    contradict Ht.
+    discriminate.
   } {
     (* EMS_WithRolesAll *)
-    split. {
-      intros Ht.
-      unfold exprMatchSubjectEvalF in Ht.
-      constructor.
-      apply RoleSets.subset_2.
-      intuition.
-    } {
-      intros Ht.
-      symmetry.
-      apply RoleSets.subset_1.
-      inversion Ht.
-      intuition.
-    }
+    intros Ht.
+    intros Hcontra.
+    rewrite <- (exprMatchSubjectEvalEquivalent_RF_T _ _ Hcontra) in Ht.
+    contradict Ht; discriminate.
   } {
     (* EMS_WithRolesAny *)
-    split. {
-      intros Ht.
-      unfold exprMatchSubjectEvalF in Ht.
-      constructor.
-      symmetry in Ht.
-
-      assert (
-        SetoidList.compat_bool
-          RoleSets.E.eq (fun x : RoleSets.elt => RoleSets.mem x (sRoles s))
-      ) as Hsetcomp. {
-        unfold SetoidList.compat_bool.
-        unfold Morphisms.Proper.
-        unfold Morphisms.respectful.
-        intros x y Heq.
-        rewrite Heq.
-        reflexivity.
-      }
-
-      pose proof (RoleSets.exists_2 Hsetcomp Ht) as [x [H0 H1]].
-      exists x.
-      intuition.
-    } {
-      intros Ht.
-      symmetry.
-      inversion Ht as [ | |s0 r0 HHt| | ].
-      subst s0.
-      subst r0.
-      simpl.
-      assert (
-        RoleSets.Exists 
-          (fun x : RoleSets.elt => RoleSets.mem x (sRoles s) = true) r
-      ) as Hex. {
-        unfold RoleSets.Exists.
-        destruct HHt as [y [Hy0 Hy1]].
-        exists y.
-        intuition.
-      }
-
-      assert (
-        SetoidList.compat_bool
-          RoleSets.E.eq (fun x : RoleSets.elt => RoleSets.mem x (sRoles s))
-      ) as Hsetcomp. {
-        unfold SetoidList.compat_bool.
-        unfold Morphisms.Proper.
-        unfold Morphisms.respectful.
-        intros x y Heq.
-        rewrite Heq.
-        reflexivity.
-      }
-
-      apply (RoleSets.exists_1 Hsetcomp Hex).
-    }
+    intros Ht.
+    intros Hcontra.
+    rewrite <- (exprMatchSubjectEvalEquivalent_RF_T _ _ Hcontra) in Ht.
+    contradict Ht; discriminate.
   } {
     (* EMS_And *)
-    split. {
-      intros Ht.
+    intros Ht.
+    intros Hcontra.
+    rewrite <- (exprMatchSubjectEvalEquivalent_RF_T _ _ Hcontra) in Ht.
+    contradict Ht; discriminate.
+  } {
+    (* EMS_Or *)
+    intros Ht.
+    intros Hcontra.
+    rewrite <- (exprMatchSubjectEvalEquivalent_RF_T _ _ Hcontra) in Ht.
+    contradict Ht; discriminate.
+  }
+Qed.
+
+Lemma exprMatchSubjectEvalEquivalent_RF_F : forall s e,
+  ~exprMatchSubjectEvalR s e -> false = exprMatchSubjectEvalF s e.
+Proof.
+  intros s e.
+  induction e as [
+    |
+    |
+    |
+    |es Hes
+    |es Hes
+  ] using exprMatchSubject_extendedInd. {
+    (* EMS_False *)
+    intros Ht.
+    reflexivity.
+  } {
+    (* EMS_True *)
+    intros Ht.
+    contradict Ht.
+    constructor.
+  } {
+    (* EMS_WithRolesAll *)
+    intros Ht.
+    simpl.
+    assert (~RoleSets.Subset r (sRoles s)) as Hns. {
+      intros Hcontra.
+      apply Ht.
       constructor.
-      simpl in Ht.
-      pose proof (Bool.andb_true_eq _ _ Ht) as [HT0 HT1].
-      intuition.
+      exact Hcontra.
+    }
+    symmetry.
+    rewrite <- roleSubsetFalse.
+    intuition.
+  } {
+    (* EMS_WithRolesAny *)
+    intros Ht.
+    symmetry.
+    intuition.
+    simpl.
+
+    assert (
+      SetoidList.compat_bool
+        RoleSets.E.eq (fun x : RoleSets.elt => RoleSets.mem x (sRoles s))
+    ) as Hsetcomp. {
+      unfold SetoidList.compat_bool.
+      unfold Morphisms.Proper.
+      unfold Morphisms.respectful.
+      intros x y Heq.
+      rewrite Heq.
+      reflexivity.
+    }
+
+    rewrite <- (roleExistsFalse r _ Hsetcomp).
+    intro Hcontra.
+    apply Ht.
+    constructor.
+    inversion Hcontra as [z [Hz0 Hz1]].
+    exists z.
+    intuition.
+  } {
+    (* EMS_And *)
+    intros Ht.
+    destruct (exprMatchSubjectEvalF s (EMS_And es)) eqn:H. {
+      symmetry in H.
+      rewrite exprMatchSubjectEvalEquivalentT in H.
+      contradiction.
     } {
-      intros Ht.
-      inversion Ht as [ | | |s0 e2 e3 He| ].
-      subst s0.
-      subst e2.
-      subst e3.
-      rewrite <- He0 in He.
-      rewrite <- He1 in He.
-      symmetry.
-      simpl.
-      rewrite Bool.andb_true_iff.
-      intuition.
+      reflexivity.
     }
   } {
     (* EMS_Or *)
-    split. {
-      intros Ht.
-      constructor.
-      simpl in Ht.
-      symmetry in Ht.
-      pose proof (Bool.orb_prop _ _ Ht) as Hb.
-      destruct Hb as [Hb0|Hb1]. {
-        symmetry in Hb0.
-        rewrite He0 in Hb0.
-        intuition.
-      } {
-        symmetry in Hb1.
-        rewrite He1 in Hb1.
-        intuition.
-      }
+    intros Ht.
+    destruct (exprMatchSubjectEvalF s (EMS_Or es)) eqn:H. {
+      symmetry in H.
+      rewrite exprMatchSubjectEvalEquivalentT in H.
+      contradiction.
     } {
-      intros Ht.
-      simpl.
-      symmetry.
-      rewrite Bool.orb_true_iff.
-      inversion Ht as [ | | |  |s0 e2 e3 He].
-      subst s0.
-      subst e2.
-      subst e3.
-      intuition.
+      reflexivity.
     }
   }
 Qed.
@@ -235,157 +497,9 @@ Qed.
 Theorem exprMatchSubjectEvalEquivalentF : forall s e,
   false = exprMatchSubjectEvalF s e <-> ~exprMatchSubjectEvalR s e.
 Proof.
-  intros s e.
-  induction e as [
-    |
-    |r
-    |r
-    |e0 He0 e1 He1
-    |e0 He0 e1 He1
-  ]. {
-    (* EMS_False *)
-    split. {
-      intros Ht H; inversion H.
-    } {
-      intros Ht; reflexivity.
-    }
-  } {
-    (* EMS_True *)
-    split. {
-      intros Ht; inversion Ht.
-    } {
-      intros Ht.
-      intuition.
-      assert (exprMatchSubjectEvalR s EMS_True) by constructor.
-      contradiction.
-    }
-  } {
-    (* EMS_WithRolesAll *)
-    split. {
-      intros Ht.
-      unfold exprMatchSubjectEvalF in Ht.
-      intros H.
-      inversion H as [ |s0 r0 Hsub| | | ].
-      subst s0.
-      subst r0.
-      pose proof (RoleSets.subset_1 Hsub) as Hsub2.
-      rewrite <- Ht in Hsub2.
-      contradict Hsub2; discriminate.
-    } {
-      intros Ht.
-      simpl.
-      assert (~RoleSets.Subset r (sRoles s)) as Hns. {
-        intros Hcontra.
-        apply Ht.
-        constructor.
-        exact Hcontra.
-      }
-      symmetry.
-      rewrite <- roleSubsetFalse.
-      intuition.
-    }
-  } {
-    (* EMS_WithRolesAny *)
-    split. {
-      intros Ht.
-      unfold exprMatchSubjectEvalF in Ht.
-
-      assert (
-        SetoidList.compat_bool
-          RoleSets.E.eq (fun x : RoleSets.elt => RoleSets.mem x (sRoles s))
-      ) as Hsetcomp. {
-        unfold SetoidList.compat_bool.
-        unfold Morphisms.Proper.
-        unfold Morphisms.respectful.
-        intros x y Heq.
-        rewrite Heq.
-        reflexivity.
-      }
-
-      symmetry in Ht.
-      rewrite <- (roleExistsFalse r _ Hsetcomp) in Ht.
-      unfold RoleSets.Exists in Ht.
-
-      intros H.
-      inversion H as [ | |s0 r0 Hsub| | ].
-      subst s0.
-      subst r0.
-
-      inversion Hsub as [y [Hy0 Hy1]].
-      rewrite RoleSetsFacts.mem_iff in Hy1.
-      intuition.
-      apply Ht.
-      exists y.
-      intuition.
-    } {
-      intros Ht.
-      symmetry.
-      intuition.
-      simpl.
-
-      assert (
-        SetoidList.compat_bool
-          RoleSets.E.eq (fun x : RoleSets.elt => RoleSets.mem x (sRoles s))
-      ) as Hsetcomp. {
-        unfold SetoidList.compat_bool.
-        unfold Morphisms.Proper.
-        unfold Morphisms.respectful.
-        intros x y Heq.
-        rewrite Heq.
-        reflexivity.
-      }
-
-      rewrite <- (roleExistsFalse r _ Hsetcomp).
-      intro Hcontra.
-      apply Ht.
-      constructor.
-      inversion Hcontra as [z [Hz0 Hz1]].
-      exists z.
-      intuition.
-    }
-  } {
-    (* EMS_And *)
-    split. {
-      intros Ht.
-      intros Hcontra.
-      inversion Hcontra as [ | | |s0 e2 e3 [Hf0 Hf1]| ].
-      subst s0.
-      subst e2.
-      subst e3.
-      simpl in Ht.
-      destruct (Bool.andb_false_elim _ _ (eq_sym Ht)); intuition.
-    } {
-      intros Ht.
-      destruct (exprMatchSubjectEvalF s (EMS_And e0 e1)) eqn:H. {
-        symmetry in H.
-        rewrite exprMatchSubjectEvalEquivalentT in H.
-        contradiction.
-      } {
-        reflexivity.
-      }
-    }
-  } {
-    (* EMS_Or *)
-    split. {
-      intros Ht.
-      intros Hcontra.
-      inversion Hcontra as [ | | |s0 e2 e3 [Hf0 Hf1]| ].
-      subst s0.
-      subst e2.
-      subst e3.
-      simpl in Ht.
-      destruct (Bool.orb_false_elim _ _ (eq_sym Ht)); intuition.
-    } {
-      intros Ht.
-      destruct (exprMatchSubjectEvalF s (EMS_Or e0 e1)) eqn:H. {
-        symmetry in H.
-        rewrite exprMatchSubjectEvalEquivalentT in H.
-        contradiction.
-      } {
-        reflexivity.
-      }
-    }
-  }
+  split.
+  apply exprMatchSubjectEvalEquivalent_FR_F.
+  apply exprMatchSubjectEvalEquivalent_RF_F.
 Qed.
 
 (** The evaluation relation is decidable. *)
